AwesomeDashboards/Grafana.lean
@@ -31,14 +31,14 @@ inductive FieldConfigOverrideMatcher
 | byName (name: String)
 
 instance : Lean.ToJson FieldConfigOverrideMatcher where
-  toJson := fun t => match t with 
+  toJson := fun t => match t with
   | .byName n => Lean.Json.mkObj [⟨"id", Lean.Json.str "byName"⟩, ⟨"options", Lean.Json.str n⟩]
 
 inductive FieldConfigOverrideProperty
 | unit (value: String)
 
 instance : Lean.ToJson FieldConfigOverrideProperty where
-  toJson := fun t => match t with 
+  toJson := fun t => match t with
   | .unit v => Lean.Json.mkObj [⟨"id", Lean.Json.str "unit"⟩, ⟨"value", Lean.Json.str v⟩]
 
 structure FieldConfigOverride where
@@ -71,7 +71,7 @@ inductive GrafanaPanelTransformation
 | organize (options: GrafanaPanelOrganizeOptions)
 
 instance : Lean.ToJson GrafanaPanelTransformation where
-  toJson := fun t => match t with 
+  toJson := fun t => match t with
   | .seriesToColumns o => Lean.Json.mkObj [⟨"id", Lean.Json.str "seriesToColumns"⟩, ⟨"options", Lean.toJson o⟩]
   | .organize o => Lean.Json.mkObj [⟨"id", Lean.Json.str "organize"⟩, ⟨"options", Lean.toJson o⟩]
 
@@ -99,22 +99,22 @@ structure GrafanaDashboard where
 
 def myDatasource : GrafanaPanelDatasource := { type := "prometheus", uid := "OoN46punz" }
 
-def myGrafanaDashboard : GrafanaDashboard := { 
+def myGrafanaDashboard : GrafanaDashboard := {
   id := Option.none, uuid := "lBf76pX7k", title := "My Dashboard", tags := [], schemaVersion := 36, panels := [
     {
-      type := "text", 
-      datasource := { type := "prometheus", uid := "OoN46punz" }, 
-      context := "Hello world", 
-      title := "", 
+      type := "text",
+      datasource := { type := "prometheus", uid := "OoN46punz" },
+      context := "Hello world",
+      title := "",
       gridPos := { x := 0, y := 0, w := 12, h := 5 },
       targets := none,
       fieldConfig := { defaults := { unit := "none" }, overrides := []}
     },
     {
-      type := "timeseries", 
-      datasource := { type := "prometheus", uid := "OoN46punz" }, 
-      context := "Hello world", 
-      title := "", 
+      type := "timeseries",
+      datasource := { type := "prometheus", uid := "OoN46punz" },
+      context := "Hello world",
+      title := "",
       gridPos := { x := 0, y := 12, w := 12, h := 5 } ,
       targets := some [{
         datasource := myDatasource
@@ -131,42 +131,62 @@ def metricUnitToGrafanaUnit (u : MetricUnit) : String := match u with
   | (MetricUnit.seconds) => "s"
   | _ => "locale"
 
+/-- mapI is like map except that the map function is also passed the index of the element. -/
 def mapI (f : α → Nat → β) : Nat → List α → List β
   | _, []    => []
   | n, a::as => f a n :: mapI f (n+1) as
 
+def unsafeTemplatedInstantVectorToGrafanaExpr {t: InstantVectorType} (v: UnsafeTemplatedInstantVector t) : String := match v with
+| .selector value_vars literal_equal_selectors key_value_vars =>
+    let sls' := value_vars.map (λs => s.fst ++ "=\"$" ++ s.snd ++ "\"")
+    let lits' := literal_equal_selectors.map (λl => l.fst ++ "=\"" ++ l.snd ++ "\"")
+    let key_values_vars' := key_value_vars.map (λkvs => "$" ++ kvs)
+    "{" ++ (joinSep (sls' ++ lits' ++ key_values_vars') ", ") ++ "}"
+| .add_vector x y => s!"{unsafeTemplatedInstantVectorToGrafanaExpr x} + {unsafeTemplatedInstantVectorToGrafanaExpr y}"
+
 def panelToGrafanaPanel {e : Environment} (p : @Panel e) (pos : GrafanaPanelGridPos) : GrafanaPanel := match p with
-| Panel.graph g =>  { 
-  type := "timeseries", 
+| Panel.graph g =>  {
+  type := "timeseries",
   title := "",
   gridPos := pos,
   context := "Hello world",
-  description := g.promql.helpString,
+  description := match g.promql with
+    | .inl promql => .some promql.helpString
+    | .inr _ => .none
   datasource := myDatasource,
   targets := some [
-    { datasource := myDatasource, expr := g.promql.v.toString, refId := "A", legendFormat := g.legendFormat }
+    {
+      datasource := myDatasource,
+      expr := match g.promql with
+        | .inl promql => promql.v.toString
+        | .inr promql => unsafeTemplatedInstantVectorToGrafanaExpr promql
+      refId := "A",
+      legendFormat := g.legendFormat
+    }
   ],
   fieldConfig := {
     defaults := {
-      unit := match unitOf e g.promql.v with
-        | (some m) => metricUnitToGrafanaUnit m
-        | _ => "none"
+      unit := match g.promql with
+        | .inl promql => match unitOf e promql.v with
+          | (some m) => metricUnitToGrafanaUnit m
+          | _ => "none"
+        | .inr _ => "none"
     },
     overrides := []
   }
 }
 | Panel.table t => {
-      type := "table", 
-      datasource := { type := "prometheus", uid := "OoN46punz" }, 
-      context := "Hello table", 
-      title := t.name, 
+      type := "table",
+      datasource := { type := "prometheus", uid := "OoN46punz" },
+      context := "Hello table",
+      title := t.name,
       gridPos := pos,
-      targets := some $ mapI (fun c i => 
+      targets := some $ mapI (fun c i =>
         { datasource := myDatasource, expr := c.promql.v.toString, refId := String.mk [Char.ofNat (65+i)], format := "table", instant := true, range := false }
       ) 0 t.columns,
       transformations := .some [
         .seriesToColumns { byField := t.joinLabel },
-        .organize { 
+        .organize {
           excludeByName := Lean.HashMap.ofList $ (
             if t.columns.length = 1 then
               [⟨"Time", true⟩]
@@ -181,10 +201,10 @@ def panelToGrafanaPanel {e : Environment} (p : @Panel e) (pos : GrafanaPanelGrid
               List.foldl (·++·) [] $ mapI (fun c i => List.map (⟨s!"{·} {i+1}", true⟩) $ c.promql.labels.filter (not ∘ (c.additionalLabels.contains ·))) 0 t.columns
           ),
           renameByName := Lean.HashMap.ofList (
-            if h: t.columns.length = 1 then 
+            if h: t.columns.length = 1 then
               let h' : 0 < List.length t.columns := by simp[h];
               [⟨"Value", (t.columns[0]).name⟩]
-            else 
+            else
               mapI (fun c i => ⟨s!"Value #{String.mk [Char.ofNat (65+i)]}", c.name⟩) 0 t.columns
           )
         }
